txn-data-consistency/CCv_Eiger_Port_plus_proof.thy
@@ -15,10 +15,10 @@ lemma wtxns_dom_eq_empty_conv [simp]: "wtxns_dom wtxns = {} \<longleftrightarrow
 lemma wtxns_domI1: "wtxns t = Prep ts v \<Longrightarrow> t \<in> wtxns_dom wtxns"
   by (simp add: wtxns_dom_def)
 
-lemma wtxns_domI2: "wtxns t = Commit cts v rs \<Longrightarrow> t \<in> wtxns_dom wtxns"
+lemma wtxns_domI2: "wtxns t = Commit cts v rs deps \<Longrightarrow> t \<in> wtxns_dom wtxns"
   by (simp add: wtxns_dom_def)
 
-lemma wtxns_domD: "t \<in> wtxns_dom wtxns \<Longrightarrow> (\<exists>ts v. wtxns t = Prep ts v) \<or> (\<exists>cts v rs. wtxns t = Commit cts v rs)"
+lemma wtxns_domD: "t \<in> wtxns_dom wtxns \<Longrightarrow> (\<exists>ts v. wtxns t = Prep ts v) \<or> (\<exists>cts v rs deps. wtxns t = Commit cts v rs deps)"
   by (cases "wtxns t") (auto simp add: wtxns_dom_def)
 
 lemma wtxns_domIff [iff, simp del, code_unfold]: "t \<in> wtxns_dom wtxns \<longleftrightarrow> wtxns t \<noteq> No_Ver"
@@ -41,13 +41,13 @@ lemma insert_prep_wtxns_dom:
   unfolding wtxns_dom_def by auto
 
 lemma insert_commit_wtxns_dom:
-  "wtxns t = Commit cts v rs \<Longrightarrow> insert t (wtxns_dom wtxns) = wtxns_dom wtxns"
+  "wtxns t = Commit cts v rs deps \<Longrightarrow> insert t (wtxns_dom wtxns) = wtxns_dom wtxns"
   unfolding wtxns_dom_def by auto
 
 
 subsection \<open>wtxns_vran lemmas\<close>
 
-lemma wtxns_vranI1: "wtxns t = Commit cts v rs \<Longrightarrow> v \<in> wtxns_vran wtxns"
+lemma wtxns_vranI1: "wtxns t = Commit cts v rs deps \<Longrightarrow> v \<in> wtxns_vran wtxns"
   apply (simp add: wtxns_vran_def)
   by (metis ver_state.sel(4) wtxns_domI2)
 
@@ -59,7 +59,7 @@ lemma wtxns_vran_empty [simp]: "wtxns_vran wtxns_emp = {}"
   by (auto simp: wtxns_vran_def)
 
 lemma wtxns_vran_map_upd [simp]:  "wtxns t = No_Ver \<Longrightarrow>
-  wtxns_vran (wtxns (t := Commit cts v rs)) = insert v (wtxns_vran wtxns)"
+  wtxns_vran (wtxns (t := Commit cts v rs deps)) = insert v (wtxns_vran wtxns)"
   by (auto simp add: wtxns_vran_def)
 
 lemma finite_wtxns_vran:
@@ -75,7 +75,7 @@ qed
       
 subsection \<open>wtxns_rsran lemmas\<close>
 
-lemma wtxns_rsranI: "wtxns t = Commit cts v rs \<Longrightarrow> rs \<subseteq> wtxns_rsran wtxns"
+lemma wtxns_rsranI: "wtxns t = Commit cts v rs deps \<Longrightarrow> rs \<subseteq> wtxns_rsran wtxns"
   apply (simp add: wtxns_rsran_def)
   by (metis (mono_tags, lifting) Sup_upper get_rs.simps(3) mem_Collect_eq wtxns_domI2)
 
@@ -87,16 +87,16 @@ lemma wtxns_rsran_map_upd1 [simp]:  "wtxns t = No_Ver \<Longrightarrow>
   by (auto simp add: wtxns_rsran_def)
 
 lemma wtxns_rsran_map_upd2 [simp]:  "wtxns t = No_Ver \<Longrightarrow>
-  wtxns_rsran (wtxns (t := Commit cts v rs)) = rs \<union> (wtxns_rsran wtxns)"
+  wtxns_rsran (wtxns (t := Commit cts v rs deps)) = rs \<union> (wtxns_rsran wtxns)"
   by (auto simp add: wtxns_rsran_def)
 
 lemma wtxns_rsran_map_upd3 [simp]:  "is_prepared (wtxns t) \<Longrightarrow>
-  wtxns_rsran (wtxns (t := Commit cts v rs)) = rs \<union> (wtxns_rsran wtxns)"
+  wtxns_rsran (wtxns (t := Commit cts v rs deps)) = rs \<union> (wtxns_rsran wtxns)"
   apply (auto simp add: wtxns_rsran_def)
   by (metis empty_iff get_rs.simps(2) is_prepared.elims(2) wtxns_domIff)
 
-lemma wtxns_rsran_map_upd4 [simp]:  "wtxns t_wr = Commit cts v rs \<Longrightarrow>
-  wtxns_rsran (wtxns (t_wr := Commit cts v (insert t rs))) = insert t (wtxns_rsran wtxns)"
+lemma wtxns_rsran_map_upd4 [simp]:  "wtxns t_wr = Commit cts v rs deps \<Longrightarrow>
+  wtxns_rsran (wtxns (t_wr := Commit cts v (insert t rs) deps)) = insert t (wtxns_rsran wtxns)"
   apply (auto simp add: wtxns_rsran_def)
   apply (metis get_rs.simps(3) wtxns_domI2)
   by (metis get_rs.simps(3) insertI2 wtxns_domIff)
@@ -146,22 +146,26 @@ lemma add_to_readerset_prep_inv:
   by (simp add: add_to_readerset_def split: ver_state.split)
 
 lemma add_to_readerset_commit:
-  "add_to_readerset wtxns t t' t'' = Commit cts v rs \<Longrightarrow> \<exists>rs'. wtxns t'' = Commit cts v rs'"
+  "add_to_readerset wtxns t t' t'' = Commit cts v rs deps \<Longrightarrow>
+    \<exists>rs'. wtxns t'' = Commit cts v rs' deps"
   apply (simp add: add_to_readerset_def)
   by (cases "wtxns t'"; cases "t'' = t'"; auto)
 
 lemma add_to_readerset_commit_subset:
-  "add_to_readerset wtxns t t' t'' = Commit cts v rs \<Longrightarrow> \<exists>rs'. wtxns t'' = Commit cts v rs' \<and> rs' \<subseteq> rs"
+  "add_to_readerset wtxns t t' t'' = Commit cts v rs deps \<Longrightarrow>
+    \<exists>rs'. wtxns t'' = Commit cts v rs' deps \<and> rs' \<subseteq> rs"
   apply (simp add: add_to_readerset_def)
   by (cases "wtxns t'"; cases "t'' = t'"; auto)
 
 lemma add_to_readerset_commit':
-  "wtxns t'' = Commit cts v rs' \<Longrightarrow> \<exists>rs. add_to_readerset wtxns t t' t'' = Commit cts v rs"
+  "wtxns t'' = Commit cts v rs' deps \<Longrightarrow>
+    \<exists>rs. add_to_readerset wtxns t t' t'' = Commit cts v rs deps"
   apply (simp add: add_to_readerset_def)
   by (cases "wtxns t'"; cases "t'' = t'"; auto)
 
 lemma add_to_readerset_commit'_subset:
-  "wtxns t'' = Commit cts v rs' \<Longrightarrow> \<exists>rs. add_to_readerset wtxns t t' t'' = Commit cts v rs \<and> rs' \<subseteq> rs"
+  "wtxns t'' = Commit cts v rs' deps \<Longrightarrow>
+    \<exists>rs. add_to_readerset wtxns t t' t'' = Commit cts v rs deps \<and> rs' \<subseteq> rs"
   apply (simp add: add_to_readerset_def)
   by (cases "wtxns t'"; cases "t'' = t'"; auto)
 
@@ -179,14 +183,14 @@ lemma ran_map_upd_None_finite:
 
 lemma pending_wtxns_ts_empty:
   "pending_wtxns_ts (wtxn_state (svrs s k)) = {} \<longleftrightarrow>
-    (\<forall>t. \<exists>cts v rs. wtxn_state (svrs s k) t \<in> {No_Ver, Commit cts v rs})"
+    (\<forall>t. \<exists>cts v rs deps. wtxn_state (svrs s k) t \<in> {No_Ver, Commit cts v rs deps})"
   apply (auto simp add: pending_wtxns_ts_def)
   apply (metis get_rs.elims)
   by (metis ver_state.distinct(1) ver_state.distinct(5))
 
 lemma pending_wtxns_ts_non_empty:
   assumes "wtxn_state (svrs s k) t \<noteq> No_Ver"
-    and "\<forall>cts v rs. wtxn_state (svrs s k) t \<noteq> Commit cts v rs"
+    and "\<forall>cts v rs deps. wtxn_state (svrs s k) t \<noteq> Commit cts v rs deps"
   shows "pending_wtxns_ts (wtxn_state (svrs s k)) \<noteq> {}"
   using assms apply (auto simp add: pending_wtxns_ts_def)
   by (meson get_rs.elims)
@@ -206,7 +210,7 @@ lemma finite_pending_wtxns_adding:
 
 lemma finite_pending_wtxns_removing: 
   assumes "finite (pending_wtxns_ts (wtxn_state (svrs s k)))"
-  shows "finite (pending_wtxns_ts ((wtxn_state (svrs s k)) (t := Commit cts v rs)))"
+  shows "finite (pending_wtxns_ts ((wtxn_state (svrs s k)) (t := Commit cts v rs deps)))"
   using assms
   by (auto simp add: finite_nat_set_iff_bounded_le pending_wtxns_ts_def)
 
@@ -217,7 +221,7 @@ lemma pending_wtxns_adding_ub:
 
 lemma pending_wtxns_removing_ub:
   assumes "\<forall>ts \<in> pending_wtxns_ts (wtxn_state (svrs s k)). ts \<le> clk"
-  shows "\<forall>ts \<in> pending_wtxns_ts ((wtxn_state (svrs s k)) (t := Commit cts v rs)). ts \<le> clk"
+  shows "\<forall>ts \<in> pending_wtxns_ts ((wtxn_state (svrs s k)) (t := Commit cts v rs deps)). ts \<le> clk"
   using assms by (auto simp add: finite_nat_set_iff_bounded_le pending_wtxns_ts_def)
 
 lemma pending_wtxns_rtxn:
@@ -234,9 +238,9 @@ lemma pending_wtxns_adding:
 
 lemma pending_wtxns_removing:
   assumes "wtxn_state (svrs s k) t = Prep clk v"
-  shows "pending_wtxns_ts ((wtxn_state (svrs s k)) (t := Commit cts v rs)) =
+  shows "pending_wtxns_ts ((wtxn_state (svrs s k)) (t := Commit cts v rs deps)) =
           pending_wtxns_ts (wtxn_state (svrs s k)) \<or>
-         pending_wtxns_ts ((wtxn_state (svrs s k)) (t := Commit cts v rs)) =
+         pending_wtxns_ts ((wtxn_state (svrs s k)) (t := Commit cts v rs deps)) =
           Set.remove clk (pending_wtxns_ts (wtxn_state (svrs s k)))"
   using assms apply (auto simp add: pending_wtxns_ts_def)
   by (metis ver_state.inject(1))+
@@ -250,32 +254,32 @@ lemma other_prep_t_inv:
 
 lemma get_view_inv:
   assumes "state_trans s e s'"
-    and "\<forall>cl keys. e \<noteq> RInvoke cl keys" and "\<forall>k t v cts. e \<noteq> CommitW k t v cts"
+    and "\<forall>cl keys. e \<noteq> RInvoke cl keys" and "\<forall>k t v cts deps. e \<noteq> CommitW k t v cts deps"
   shows "get_view s' cl = get_view s cl"
   using assms
 proof (induction e)
   case (RegR x1 x2 x3 x4)
   then show ?case apply (auto simp add: tps_trans_defs get_view_def)
-    apply (rule ext, auto del: disjE split: if_split_asm)
+    apply (auto del: disjE split: if_split_asm)
     apply (metis add_to_readerset_commit)
-    by (meson add_to_readerset_commit')
+    apply (metis add_to_readerset_commit)
+    by (meson add_to_readerset_commit')+
 next
   case (PrepW x1 x2 x3)
-  then show ?case apply (auto simp add: tps_trans_defs get_view_def)
-    by (rule ext, auto)
+  then show ?case apply (auto simp add: tps_trans_defs get_view_def) sorry
 qed (auto simp add: tps_trans_defs get_view_def)
 
 lemma get_view_wcommit_inv:
-  assumes "wtxn_state (svrs s' k) = (wtxn_state (svrs s k)) (t := Commit cts v {})"
+  assumes "wtxn_state (svrs s' k) = (wtxn_state (svrs s k)) (t := Commit cts v {} deps)"
     and "wtxn_state (svrs s k) t = Prep ts v"
-    and "txn_state (cls s (get_cl_wtxn t)) = WtxnCommit cts kv_map"
+    and "txn_state (cls s (get_cl_wtxn t)) = WtxnCommit cts kv_map deps"
     and "get_cl_wtxn t \<noteq> cl"
     and "\<forall>k'. k' \<noteq> k \<longrightarrow> svrs s' k' = svrs s k'"
     and "gst (cls s' cl) = gst (cls s cl)"
   shows "get_view s' cl = get_view s cl"
   using assms
   apply (simp add: get_view_def add_to_readerset_def)
-  apply (rule ext, auto del: disjE)
+  apply (auto del: disjE)
   subgoal for k' apply (cases "k' = k"; simp split: if_split_asm) oops
   (* show cts > rts *)
 
@@ -285,22 +289,22 @@ lemma get_view_other_cl:
   shows "get_view s' cl' = get_view s cl'"
   using assms
   apply (simp add: get_view_def)
-  apply (rule ext, rule Collect_eqI, auto) oops
+  apply (rule Collect_eqI, auto) oops
 
 
 lemma view_of_prefix:
   assumes "\<And>k. prefix (corder k) (corder' k)"
     and "\<And>k. distinct (corder' k)"
-    and "\<And>k. u k \<subseteq> set (corder k)"
+    and "\<And>k. u `` {k} \<subseteq> set (corder k)"
   shows "view_of corder u = view_of corder' u"
   unfolding view_of_def
 proof (rule ext, rule Collect_eqI, rule iffI)
   fix k pos
-  assume *: "\<exists>t. pos = (THE i. i < length (corder k) \<and> corder k ! i = t) \<and> t \<in> u k \<and> t \<in> set (corder k)"
-  show "\<exists>t. pos = (THE i. i < length (corder' k) \<and> corder' k ! i = t) \<and> t \<in> u k \<and> t \<in> set (corder' k)"
+  assume *: "\<exists>t. pos = (THE i. i < length (corder k) \<and> corder k ! i = t) \<and> (k, t) \<in> u \<and> t \<in> set (corder k)"
+  show "\<exists>t. pos = (THE i. i < length (corder' k) \<and> corder' k ! i = t) \<and> (k, t) \<in> u \<and> t \<in> set (corder' k)"
   proof -
     from assms(1) obtain zs where p: "corder k @ zs = corder' k" using prefixE by metis
-    from * obtain tid where **: "tid \<in> u k" "tid \<in> set (corder k)"
+    from * obtain tid where **: "(k, tid) \<in> u" "tid \<in> set (corder k)"
       "pos = (THE i. i < length (corder k) \<and> corder k ! i = tid)" by blast
     from \<open>tid \<in> set (corder k)\<close> obtain i
       where the_i: "i < length (corder k) \<and> corder k ! i = tid" by (meson in_set_conv_nth)
@@ -320,11 +324,11 @@ proof (rule ext, rule Collect_eqI, rule iffI)
   qed
 next
   fix k pos
-  assume *: "\<exists>t. pos = (THE i. i < length (corder' k) \<and> corder' k ! i = t) \<and> t \<in> u k \<and> t \<in> set (corder' k)"
-  show "\<exists>t. pos = (THE i. i < length (corder k) \<and> corder k ! i = t) \<and> t \<in> u k \<and> t \<in> set (corder k)"
+  assume *: "\<exists>t. pos = (THE i. i < length (corder' k) \<and> corder' k ! i = t) \<and> (k, t) \<in> u \<and> t \<in> set (corder' k)"
+  show "\<exists>t. pos = (THE i. i < length (corder k) \<and> corder k ! i = t) \<and> (k, t) \<in> u \<and> t \<in> set (corder k)"
   proof -
     from assms(1) obtain zs where p: "corder k @ zs = corder' k" using prefixE by metis
-    from * obtain tid where **: "tid \<in> u k" "tid \<in> set (corder' k)"
+    from * obtain tid where **: "(k, tid) \<in> u" "tid \<in> set (corder' k)"
       "pos = (THE i. i < length (corder' k) \<and> corder' k ! i = tid)" by blast
     from \<open>tid \<in> set (corder' k)\<close> obtain i' where the_i':"i' < length (corder' k) \<and> corder' k ! i' = tid"
       by (meson in_set_conv_nth)
@@ -435,7 +439,7 @@ next
       apply (auto simp add: Pend_Wt_UB_def tps_trans_defs pending_wtxns_ts_def)
       by (meson le_Suc_eq max.coboundedI1)
   next
-    case (CommitW x1 x2 x3 x4)
+    case (CommitW x1 x2 x3 x4 x5)
     then show ?case
       apply (auto simp add: Pend_Wt_UB_def tps_trans_defs pending_wtxns_ts_def split: if_split_asm)
       by (meson le_Suc_eq max.coboundedI1 notin_set_remove1)
@@ -518,7 +522,7 @@ next
     case (PrepW x1 x2 x3)
     then show ?case by (auto simp add: Pend_Wt_LB_def tps_trans_defs pending_wtxns_adding)
   next
-    case (CommitW x1 x2 x3 x4)
+    case (CommitW x1 x2 x3 x4 x5)
     then show ?case apply (auto simp add: Pend_Wt_LB_def tps_trans_defs split: if_split_asm)
       by (meson Finite_Pend_Inv_def Min_le finite_pending_wtxns_removing reach_finitepending)
   qed(auto simp add: Pend_Wt_LB_def tps_trans_defs)
@@ -545,7 +549,7 @@ next
       pending_wtxns_adding [of s x1]
     by (cases "k = x1"; auto simp add: pending_wtxns_ts_def)
 next
-  case (CommitW x1 x2 x3 x4)
+  case (CommitW x1 x2 x3 x4 x5)
   then show ?case
     apply (auto simp add: commit_write_def Finite_Pend_Inv_def fold_pending_wtxns_fun_upd)
     by (metis Min.coboundedI Min_in Min_remove empty_iff pending_wtxns_removing is_prepared.elims(2)
@@ -583,8 +587,8 @@ next
   case (reach_trans s e s')
   then show ?case
   proof (induction e)
-    case (CommitW x1 x2 x3 x4)
-    then show ?case using lst_monotonic[of s "CommitW x1 x2 x3 x4" s' x1]
+    case (CommitW x1 x2 x3 x4 x5)
+    then show ?case using lst_monotonic[of s "CommitW x1 x2 x3 x4 x5" s' x1]
       apply (auto simp add: Lst_map_le_Lst_def tps_trans_defs)
       by (smt (z3) all_not_in_conv le_trans)
   qed (auto simp add: Lst_map_le_Lst_def tps_trans_defs)
@@ -599,7 +603,7 @@ lemma lst_map_monotonic:
 
 definition Finite_Dom_Kv_map where
   "Finite_Dom_Kv_map s cl \<longleftrightarrow>
-    (\<forall>kv_map cts. txn_state (cls s cl) \<in> {WtxnPrep kv_map, WtxnCommit cts kv_map} \<longrightarrow>
+    (\<forall>kv_map cts deps. txn_state (cls s cl) \<in> {WtxnPrep kv_map, WtxnCommit cts kv_map deps} \<longrightarrow>
       finite (dom (kv_map)))"
                                                            
 lemmas Finite_Dom_Kv_mapI = Finite_Dom_Kv_map_def[THEN iffD2, rule_format]
@@ -744,7 +748,7 @@ next
   then show ?case apply (auto simp add: Lst_Lt_Pts_def tps_trans_defs)
     by (meson add_to_readerset_prep_inv)
   next
-    case (CommitW x1 x2 x3 x4)
+    case (CommitW x1 x2 x3 x4 x5)
     then show ?case apply (auto simp add: Lst_Lt_Pts_def tps_trans_defs)
       apply (metis emptyE other_prep_t_inv)
       by (metis Finite_Pend_Inv_def Min.coboundedI finite_pending_wtxns_removing other_prep_t_inv
@@ -781,7 +785,7 @@ next
       apply (auto simp add: Kvs_Not_Emp_def tps_trans_defs)
       by (metis fun_upd_same ver_state.distinct(1))
   next
-    case (CommitW x1 x2 x3 x4)
+    case (CommitW x1 x2 x3 x4 x5)
     then show ?case
       apply (auto simp add: Kvs_Not_Emp_def tps_trans_defs)
       by (metis fun_upd_same ver_state.distinct(3))
@@ -819,7 +823,7 @@ lemma reach_kvs_of_s_not_emp [simp]: "reach tps s \<Longrightarrow> KvsOfS_Not_E
 
 
 definition Init_Ver_Inv where
-  "Init_Ver_Inv s k \<longleftrightarrow> (\<exists>rs. wtxn_state (svrs s k) T0 = Commit 0 undefined rs)"
+  "Init_Ver_Inv s k \<longleftrightarrow> (\<exists>rs. wtxn_state (svrs s k) T0 = Commit 0 undefined rs {})"
 
 lemmas Init_Ver_InvI = Init_Ver_Inv_def[THEN iffD2, rule_format]
 lemmas Init_Ver_InvE[elim] = Init_Ver_Inv_def[THEN iffD1, elim_format, rule_format]
@@ -906,7 +910,7 @@ next
     then show ?case apply (simp add: Idle_Read_Inv_def tps_trans_defs)
       by (metis get_cl_wtxn.simps(2) state_txn.distinct(3) state_txn.distinct(7))
   next
-    case (CommitW x1 x2 x3 x4)
+    case (CommitW x1 x2 x3 x4 x5)
     then show ?case apply (simp add: Idle_Read_Inv_def tps_trans_defs)
       by force
   qed (auto simp add: Idle_Read_Inv_def tps_trans_defs)
@@ -914,7 +918,7 @@ qed
 
 definition Wr_Svr_Idle where
   "Wr_Svr_Idle s \<longleftrightarrow>
-    (\<forall>cl k cts kv_map. txn_state (cls s cl) \<in> {WtxnPrep kv_map, WtxnCommit cts kv_map}
+    (\<forall>cl k cts kv_map deps. txn_state (cls s cl) \<in> {WtxnPrep kv_map, WtxnCommit cts kv_map deps}
         \<and> kv_map k = None \<longrightarrow> wtxn_state (svrs s k) (Tn (get_txn_cl s cl)) = No_Ver)"
 
 lemmas Wr_Svr_IdleI = Wr_Svr_Idle_def[THEN iffD2, rule_format]
@@ -937,7 +941,7 @@ next
     then show ?case apply (simp add: Wr_Svr_Idle_def tps_trans_defs)
       by (smt (z3) domIff get_cl_wtxn.simps(2) state_txn.distinct(11) state_txn.inject(2))
   next
-    case (CommitW x1 x2 x3 x4)
+    case (CommitW x1 x2 x3 x4 x5)
     then show ?case apply (simp add: Wr_Svr_Idle_def tps_trans_defs)
       by force
   qed (auto simp add: Wr_Svr_Idle_def tps_trans_defs, blast?)
@@ -971,15 +975,15 @@ next
     then show ?case apply (simp add: Prep_Inv_def tps_trans_defs)
       by (metis domI get_cl_wtxn.simps(2) state_txn.inject(2))
   next
-    case (CommitW x1 x2 x3 x4)
+    case (CommitW x1 x2 x3 x4 x5)
     then show ?case apply (simp add: Prep_Inv_def tps_trans_defs)
       using get_cl_wtxn.simps(2) state_txn.distinct(11) state_txn.simps(19) by force
   qed (auto simp add: Prep_Inv_def tps_trans_defs)
 qed
 
 definition Commit_Inv where
-  "Commit_Inv s \<longleftrightarrow> (\<forall>cl k cts kvm. \<exists>prep_t v rs. txn_state (cls s cl) = WtxnCommit cts kvm
-    \<longrightarrow> (k \<in> dom kvm \<longrightarrow> wtxn_state (svrs s k) (get_wtxn_cl s cl) \<in> {Prep prep_t v, Commit cts v rs}) \<and>
+  "Commit_Inv s \<longleftrightarrow> (\<forall>cl k cts kvm. \<exists>prep_t v rs deps. txn_state (cls s cl) = WtxnCommit cts kvm deps
+    \<longrightarrow> (k \<in> dom kvm \<longrightarrow> wtxn_state (svrs s k) (get_wtxn_cl s cl) \<in> {Prep prep_t v, Commit cts v rs deps}) \<and>
     (k \<notin> dom kvm \<longrightarrow> wtxn_state (svrs s k) (get_wtxn_cl s cl) = No_Ver))"
 
 lemmas Commit_InvI = Commit_Inv_def[THEN iffD2, rule_format]
@@ -996,7 +1000,7 @@ next
   proof (induction e)
     case (WCommit x1 x2 x3 x4 x5)
     then show ?case apply (simp add: Commit_Inv_def tps_trans_defs)
-      by (meson Prep_Inv_def is_prepared.elims(2) reach_prep_inv)
+      by blast
   next
     case (RegR x1 x2 x3 x4)
     then show ?case apply (simp add: Commit_Inv_def tps_trans_defs)
@@ -1007,7 +1011,7 @@ next
     then show ?case apply (simp add: Commit_Inv_def tps_trans_defs)
       by (smt (verit) fun_upd_other get_cl_wtxn.simps(2) state_txn.distinct(11))
   next
-    case (CommitW x1 x2 x3 x4)
+    case (CommitW x1 x2 x3 x4 x5)
     then show ?case apply (simp add: Commit_Inv_def tps_trans_defs)
       using fun_upd_same get_cl_wtxn.simps(2) state_txn.simps(19) ver_state.distinct(1)
         ver_state.simps(10) by force
@@ -1018,7 +1022,7 @@ qed
 definition PTid_Inv where
   "PTid_Inv s cl \<longleftrightarrow> (\<forall>k. \<forall>n < txn_sn (cls s cl).
    (wtxn_state (svrs s k) (Tn (Tn_cl n cl)) = No_Ver) \<or>
-   (rtxn_rts s (Tn_cl n cl) = None \<and> (\<exists>cts v rs. wtxn_state (svrs s k) (Tn (Tn_cl n cl)) = Commit cts v rs)))"
+   (rtxn_rts s (Tn_cl n cl) = None \<and> (\<exists>cts v rs deps. wtxn_state (svrs s k) (Tn (Tn_cl n cl)) = Commit cts v rs deps)))"
 
 lemmas PTid_InvI = PTid_Inv_def[THEN iffD2, rule_format]
 lemmas PTid_InvE[elim] = PTid_Inv_def[THEN iffD1, elim_format, rule_format]
@@ -1041,10 +1045,10 @@ next
     case (WDone x61 x62)
     then show ?case
       apply (auto simp add: tps_trans_defs PTid_Inv_def)
-      subgoal for _ _ n apply (cases "n = txn_sn (cls s x61)")
+      subgoal for _ _ _ n apply (cases "n = txn_sn (cls s x61)")
         apply (metis CFTid_Rtxn_Inv_def eq_imp_le reach_cftid_rtxn_inv)
         by (metis less_SucE)
-      subgoal for _ k apply (cases "x62 k = None")
+      subgoal for _ _ k apply (cases "x62 k = None")
         apply (metis (lifting) Wr_Svr_Idle_def insertCI less_antisym reach_wr_svr_idle)
         by (metis (no_types, lifting) domIff less_antisym)
       done
@@ -1060,7 +1064,7 @@ qed
 lemma other_sn_idle:  
   assumes "FTid_Wtxn_Inv s cl" and "PTid_Inv s cl"
     and "get_cl_txn t = cl" and "get_sn_txn t \<noteq> txn_sn (cls s cl)"
-  shows "\<And>k. \<exists>cts v rs. wtxn_state (svrs s k) (Tn t) \<in> {No_Ver, Commit cts v rs}"
+  shows "\<And>k. \<exists>cts v rs deps. wtxn_state (svrs s k) (Tn t) \<in> {No_Ver, Commit cts v rs deps}"
   using assms
   apply (auto simp add: FTid_Wtxn_Inv_def PTid_Inv_def)
   apply (cases "get_sn_txn t > txn_sn (cls s cl)")
@@ -1099,7 +1103,7 @@ qed
 
 definition Wtxn_Rtxn_None where
   "Wtxn_Rtxn_None s k \<longleftrightarrow>
-    (\<forall>cl n ts v cts rs. wtxn_state (svrs s k) (Tn (Tn_cl n cl)) \<in> {Prep ts v, Commit cts v rs}
+    (\<forall>cl n ts v cts rs deps. wtxn_state (svrs s k) (Tn (Tn_cl n cl)) \<in> {Prep ts v, Commit cts v rs deps}
        \<longrightarrow> rtxn_rts s (Tn_cl n cl) = None)"
 
 lemmas Wtxn_Rtxn_NoneI = Wtxn_Rtxn_None_def[THEN iffD2, rule_format]
@@ -1122,14 +1126,14 @@ next
       by (metis CFTid_Rtxn_Inv_def get_cl_wtxn.simps(2) get_sn_wtxn.simps(2) le_refl
           reach_cftid_rtxn_inv is_curr_wt_def)
   next
-    case (CommitW x1 x2 x3 x4)
+    case (CommitW x1 x2 x3 x4 x5)
     then show ?case apply (simp add: Wtxn_Rtxn_None_def tps_trans_defs)
       by (meson is_prepared.elims(2))
   qed (auto simp add: Wtxn_Rtxn_None_def tps_trans_defs)
 qed
 
 definition WtxnCommit_Wtxn_Cts where
-  "WtxnCommit_Wtxn_Cts s cl \<longleftrightarrow> (\<forall>cts kv_map. txn_state (cls s cl) = WtxnCommit cts kv_map
+  "WtxnCommit_Wtxn_Cts s cl \<longleftrightarrow> (\<forall>cts kv_map deps. txn_state (cls s cl) = WtxnCommit cts kv_map deps
     \<longrightarrow> wtxn_cts s (get_wtxn_cl s cl) = Some cts)"
 
 lemmas WtxnCommit_Wtxn_CtsI = WtxnCommit_Wtxn_Cts_def[THEN iffD2, rule_format]
@@ -1148,9 +1152,9 @@ qed
 
 definition Wtxn_State_Cts where
   "Wtxn_State_Cts s k \<longleftrightarrow>
-    (\<forall>t cts v rs ts kv_map. (wtxn_state (svrs s k) t = Commit cts v rs) \<or> 
+    (\<forall>t cts v rs deps ts kv_map. (wtxn_state (svrs s k) t = Commit cts v rs deps) \<or> 
       (wtxn_state (svrs s k) t = Prep ts v \<and> is_curr_wt s t \<and>
-       txn_state (cls s (get_cl_wtxn t)) = WtxnCommit cts kv_map)
+       txn_state (cls s (get_cl_wtxn t)) = WtxnCommit cts kv_map deps)
       \<longrightarrow> wtxn_cts s t = Some cts)"
 
 lemmas Wtxn_State_CtsI = Wtxn_State_Cts_def[THEN iffD2, rule_format]
@@ -1175,15 +1179,15 @@ next
     then show ?case apply (simp add: Wtxn_State_Cts_def tps_trans_defs is_curr_wt_def domI)
       by (meson add_to_readerset_commit add_to_readerset_prep_inv)
   next
-    case (CommitW x1 x2 x3 x4)
+    case (CommitW x1 x2 x3 x4 x5)
     then show ?case apply (simp add: Wtxn_State_Cts_def tps_trans_defs is_curr_wt_def domI)
       by (meson domI is_prepared.elims(2))
   qed (auto simp add: Wtxn_State_Cts_def tps_trans_defs is_curr_wt_def domI)
 qed
 
 definition FTid_notin_rs where
-  "FTid_notin_rs s cl \<longleftrightarrow> (\<forall>n k t cts v rs.  n > txn_sn (cls s cl) \<and>
-    wtxn_state (svrs s k) t = Commit cts v rs \<longrightarrow> Tn_cl n cl \<notin> rs)"
+  "FTid_notin_rs s cl \<longleftrightarrow> (\<forall>n k t cts v rs deps.  n > txn_sn (cls s cl) \<and>
+    wtxn_state (svrs s k) t = Commit cts v rs deps \<longrightarrow> Tn_cl n cl \<notin> rs)"
 
 lemmas FTid_notin_rsI = FTid_notin_rs_def[THEN iffD2, rule_format]
 lemmas FTid_notin_rsE[elim] = FTid_notin_rs_def[THEN iffD1, elim_format, rule_format]
@@ -1198,6 +1202,14 @@ next
   case (reach_trans s e s')
   then show ?case 
   proof (induction e)
+    case (RDone x1 x2 x3 x4)
+    then show ?case apply (simp add: FTid_notin_rs_def tps_trans_defs)
+      by (meson Suc_lessD)
+  next
+    case (WDone x1 x2)
+    then show ?case apply (simp add: FTid_notin_rs_def tps_trans_defs)
+      by (meson Suc_lessD)
+  next
     case (RegR x1 x2 x3 x4)
     then show ?case apply (simp add: FTid_notin_rs_def tps_trans_defs is_curr_t_def) sorry
   next
@@ -1205,7 +1217,7 @@ next
     then show ?case apply (simp add: FTid_notin_rs_def tps_trans_defs)
       by (metis)
   next
-    case (CommitW x1 x2 x3 x4)
+    case (CommitW x1 x2 x3 x4 x5)
     then show ?case apply (simp add: FTid_notin_rs_def tps_trans_defs)
       by (smt empty_iff fun_upd_other fun_upd_same state_txn.simps(19) ver_state.inject(2)
           ver_state.simps(10))
@@ -1250,8 +1262,8 @@ next
 qed
 
 definition Fresh_rd_notin_rs where
-  "Fresh_rd_notin_rs s cl k \<longleftrightarrow> (\<forall>t cts v rs. txn_state (cls s cl) = Idle \<and>
-    wtxn_state (svrs s k) t = Commit cts v rs \<longrightarrow> get_txn_cl s cl \<notin> rs)"
+  "Fresh_rd_notin_rs s cl k \<longleftrightarrow> (\<forall>t cts v rs deps. txn_state (cls s cl) = Idle \<and>
+    wtxn_state (svrs s k) t = Commit cts v rs deps \<longrightarrow> get_txn_cl s cl \<notin> rs)"
 
 lemmas Fresh_rd_notin_rsI = Fresh_rd_notin_rs_def[THEN iffD2, rule_format]
 lemmas Fresh_rd_notin_rsE[elim] = Fresh_rd_notin_rs_def[THEN iffD1, elim_format, rule_format]
@@ -1335,7 +1347,8 @@ abbreviation invariant_list_kvs where
    \<comment> \<open> KVS_Not_All_Pending s k \<and>\<close> Fresh_rd_notin_rs s cl k"
 
 abbreviation not_committing_ev where
-  "not_committing_ev e \<equiv> \<forall>cl kv_map cts sn u. e \<noteq> RDone cl kv_map sn u \<and> e \<noteq> WCommit cl kv_map cts sn u"
+  "not_committing_ev e \<equiv> \<forall>cl kvt_map kv_map cts sn u. e \<noteq> RDone cl kvt_map sn u \<and>
+    e \<noteq> WCommit cl kv_map cts sn u"
 
 lemma kvs_of_s_inv:
   assumes "state_trans s e s'"
@@ -1354,13 +1367,13 @@ next
   case (PrepW x1 x2 x3)
   then show ?case sorry
 next
-  case (CommitW x1 x2 x3 x4)
+  case (CommitW x1 x2 x3 x4 x5)
   then show ?case sorry
 qed (auto simp add: kvs_of_s_def tps_trans_defs split: ver_state.split)
 
 definition Sqn_Inv_nc where
-  "Sqn_Inv_nc s cl \<longleftrightarrow> (\<forall>cts kvm.
-    (txn_state (cls s cl) \<noteq> WtxnCommit cts kvm \<longrightarrow> (\<forall>m \<in> get_sqns (kvs_of_s s) cl. m < txn_sn (cls s cl))))"
+  "Sqn_Inv_nc s cl \<longleftrightarrow> (\<forall>cts kvm deps. txn_state (cls s cl) \<noteq> WtxnCommit cts kvm deps
+     \<longrightarrow> (\<forall>m \<in> get_sqns (kvs_of_s s) cl. m < txn_sn (cls s cl)))"
 
 lemmas Sqn_Inv_ncI = Sqn_Inv_nc_def[THEN iffD2, rule_format]
 lemmas Sqn_Inv_ncE[elim] = Sqn_Inv_nc_def[THEN iffD1, elim_format, rule_format]
@@ -1388,8 +1401,8 @@ next
 qed
 
 definition Sqn_Inv_c where
-  "Sqn_Inv_c s cl \<longleftrightarrow> (\<forall>cts kvm.
-    (txn_state (cls s cl) = WtxnCommit cts kvm \<longrightarrow> (\<forall>m \<in> get_sqns (kvs_of_s s) cl. m \<le> txn_sn (cls s cl))))"
+  "Sqn_Inv_c s cl \<longleftrightarrow> (\<forall>cts kvm deps. txn_state (cls s cl) = WtxnCommit cts kvm deps
+     \<longrightarrow> (\<forall>m \<in> get_sqns (kvs_of_s s) cl. m \<le> txn_sn (cls s cl)))"
 
 lemmas Sqn_Inv_cI = Sqn_Inv_c_def[THEN iffD2, rule_format]
 lemmas Sqn_Inv_cE[elim] = Sqn_Inv_c_def[THEN iffD1, elim_format, rule_format]
@@ -1417,7 +1430,7 @@ qed
 
 lemma t_is_fresh:
   assumes "Sqn_Inv_c s cl" and "Sqn_Inv_nc s cl"
-    and "txn_state (cls s cl) \<in> {WtxnPrep kv_map, RtxnInProg keys kv_map}"
+    and "txn_state (cls s cl) \<in> {WtxnPrep kv_map, RtxnInProg keys kvt_map}"
   shows "get_txn_cl s cl \<in> next_txids (kvs_of_s s) cl"
   using assms by (auto simp add: kvs_of_s_def next_txids_def)
 
@@ -1463,8 +1476,8 @@ next
 qed
 
 definition Gst_Lt_Cts where
-  "Gst_Lt_Cts s cl \<longleftrightarrow> (\<forall>k cts v rs. 
-      wtxn_state (svrs s k) (get_wtxn_cl s cl) = Commit cts v rs \<longrightarrow> gst (cls s cl) < cts)"
+  "Gst_Lt_Cts s cl \<longleftrightarrow> (\<forall>k cts v rs deps. 
+      wtxn_state (svrs s k) (get_wtxn_cl s cl) = Commit cts v rs deps \<longrightarrow> gst (cls s cl) < cts)"
                                                            
 lemmas Gst_Lt_CtsI = Gst_Lt_Cts_def[THEN iffD2, rule_format]
 lemmas Gst_Lt_CtsE[elim] = Gst_Lt_Cts_def[THEN iffD1, elim_format, rule_format]
@@ -1493,14 +1506,14 @@ next
     then show ?case apply (simp add: Gst_Lt_Cts_def tps_trans_defs)
       by (meson add_to_readerset_commit)
   next
-    case (CommitW x1 x2 x3 x4)
+    case (CommitW x1 x2 x3 x4 x5)
     then show ?case apply (simp add: Gst_Lt_Cts_def tps_trans_defs) sorry
   qed (auto simp add: Gst_Lt_Cts_def tps_trans_defs)
 qed
 
 
 definition Gst_lt_Cts where
-  "Gst_lt_Cts s cl \<longleftrightarrow> (\<forall>cl' cts kv_map. txn_state (cls s cl') = WtxnCommit cts kv_map
+  "Gst_lt_Cts s cl \<longleftrightarrow> (\<forall>cl' cts kv_map deps. txn_state (cls s cl') = WtxnCommit cts kv_map deps
     \<longrightarrow> gst (cls s cl) < cts)"
                                                            
 lemmas Gst_lt_CtsI = Gst_lt_Cts_def[THEN iffD2, rule_format]
@@ -1521,7 +1534,7 @@ next
     case (WCommit x1 x2 x3 x4 x5)
     then show ?case apply (auto simp add: Gst_lt_Cts_def tps_trans_defs)
       apply (cases "cl = x1"; simp) sorry
-  qed (auto simp add: Gst_lt_Cts_def tps_trans_defs)
+  qed (auto simp add: Gst_lt_Cts_def tps_trans_defs, (blast+)?)
 qed
 
 
@@ -1529,7 +1542,7 @@ subsection \<open>Invariants about commit order\<close>
 
 definition Commit_Order_Tid where
   "Commit_Order_Tid s cl \<longleftrightarrow> (case txn_state (cls s cl) of
-    WtxnCommit cts kv_map \<Rightarrow> (\<forall>k n. Tn (Tn_cl n cl) \<in> set (commit_order s k) \<longrightarrow> n \<le> txn_sn (cls s cl))
+    WtxnCommit cts kv_map deps \<Rightarrow> (\<forall>k n. Tn (Tn_cl n cl) \<in> set (commit_order s k) \<longrightarrow> n \<le> txn_sn (cls s cl))
   | _ \<Rightarrow> (\<forall>k n. Tn (Tn_cl n cl) \<in> set (commit_order s k) \<longrightarrow> n < txn_sn (cls s cl)))"
 
 lemmas Commit_Order_TidI = Commit_Order_Tid_def[THEN iffD2, rule_format]
@@ -1586,9 +1599,9 @@ qed
 
 definition Commit_Order_Sound where
   "Commit_Order_Sound s k \<longleftrightarrow> (\<forall>n cl. Tn (Tn_cl n cl) \<in> set (commit_order s k) \<longrightarrow>
-    (\<exists>cts v rs. wtxn_state (svrs s k) (Tn (Tn_cl n cl)) = Commit cts v rs) \<or> 
+    (\<exists>cts v rs deps. wtxn_state (svrs s k) (Tn (Tn_cl n cl)) = Commit cts v rs deps) \<or> 
     ((\<exists>ts v. wtxn_state (svrs s k) (Tn (Tn_cl n cl)) = Prep ts v) \<and> 
-     (\<exists>cts kv_map. txn_state (cls s cl) = WtxnCommit cts kv_map \<and> 
+     (\<exists>cts kv_map deps. txn_state (cls s cl) = WtxnCommit cts kv_map deps \<and> 
       txn_sn (cls s cl) = n \<and> k \<in> dom kv_map)))"
 
 lemmas Commit_Order_SoundI = Commit_Order_Sound_def[THEN iffD2, rule_format]
@@ -1635,7 +1648,7 @@ next
     then show ?case apply (simp add: Commit_Order_Sound_def tps_trans_defs)
       by (metis ver_state.distinct(3))
   next
-    case (CommitW x1 x2 x3 x4)
+    case (CommitW x1 x2 x3 x4 x5)
     then show ?case apply (simp add: Commit_Order_Sound_def tps_trans_defs)
       by (smt (z3) fun_upd_apply state_txn.simps(19) ver_state.simps(10))
   qed (auto simp add: Commit_Order_Sound_def tps_trans_defs)
@@ -1669,9 +1682,9 @@ lemma reach_commit_order_sound'' [simp]: "reach tps s \<Longrightarrow> Commit_O
 
 definition Commit_Order_Complete where
   "Commit_Order_Complete s k \<longleftrightarrow> (\<forall>n cl.
-    (\<exists>cts v rs. wtxn_state (svrs s k) (Tn (Tn_cl n cl)) = Commit cts v rs) \<or> 
+    (\<exists>cts v rs deps. wtxn_state (svrs s k) (Tn (Tn_cl n cl)) = Commit cts v rs deps) \<or> 
     ((\<exists>ts v. wtxn_state (svrs s k) (Tn (Tn_cl n cl)) = Prep ts v) \<and> 
-     (\<exists>cts kv_map. txn_state (cls s cl) = WtxnCommit cts kv_map \<and> txn_sn (cls s cl) = n)) \<longrightarrow>
+     (\<exists>cts kv_map deps. txn_state (cls s cl) = WtxnCommit cts kv_map deps \<and> txn_sn (cls s cl) = n)) \<longrightarrow>
     Tn (Tn_cl n cl) \<in> set (commit_order s k))"
 
 lemmas Commit_Order_CompleteI = Commit_Order_Complete_def[THEN iffD2, rule_format]
@@ -1702,49 +1715,40 @@ next
     then show ?case apply (simp add: Commit_Order_Complete_def tps_trans_defs)
       by (metis get_cl_wtxn.simps(2) state_txn.distinct(11))
   next
-    case (CommitW x1 x2 x3 x4)
+    case (CommitW x1 x2 x3 x4 x5)
     then show ?case apply (auto simp add: Commit_Order_Complete_def tps_trans_defs)
       by (metis (no_types, opaque_lifting) get_cl_wtxn.simps(2) get_sn_wtxn.simps(2) 
           is_prepared.elims(2) is_curr_wt_def)
   qed (simp_all add: Commit_Order_Complete_def tps_trans_defs)
 qed
 
-definition Commit_Order_Superset_View where
-  "Commit_Order_Superset_View s k \<longleftrightarrow> (\<forall>cl. (cl_view (cls s cl)) k \<subseteq> set (commit_order s k))"
+definition Commit_Order_Superset_Ctx where
+  "Commit_Order_Superset_Ctx s k \<longleftrightarrow> (\<forall>cl t. (k, t) \<in> cl_ctx (cls s cl) \<longrightarrow> t \<in> set (commit_order s k))"
 
-lemmas Commit_Order_Superset_ViewI = Commit_Order_Superset_View_def[THEN iffD2, rule_format]
-lemmas Commit_Order_Superset_ViewE[elim] = Commit_Order_Superset_View_def[THEN iffD1, elim_format, rule_format]
+lemmas Commit_Order_Superset_CtxI = Commit_Order_Superset_Ctx_def[THEN iffD2, rule_format]
+lemmas Commit_Order_Superset_CtxE[elim] = Commit_Order_Superset_Ctx_def[THEN iffD1, elim_format, rule_format]
 
-lemma reach_commit_order_superset_view [simp]: "reach tps s \<Longrightarrow> Commit_Order_Superset_View s k"
+lemma reach_commit_order_superset_ctx [simp]: "reach tps s \<Longrightarrow> Commit_Order_Superset_Ctx s k"
 proof(induction s rule: reach.induct)
   case (reach_init s)
   then show ?case
-    by (auto simp add: Commit_Order_Superset_View_def tps_defs view_txid_init_def)
+    by (auto simp add: Commit_Order_Superset_Ctx_def tps_defs ctx_kt_init_def)
 next
   case (reach_trans s e s')
   then show ?case
   proof (induction e)
     case (RDone x1 x2 x3 x4)
-    then show ?case apply (simp add: Commit_Order_Superset_View_def tps_trans_defs get_view_def)
-      apply (rule subsetI) subgoal for x apply (cases x)
+    then show ?case apply (auto simp add: Commit_Order_Superset_Ctx_def tps_trans_defs get_ctx_def)
+      subgoal for x apply (cases x)
         apply blast using Commit_Order_Complete_def[of s k]
-        by (smt mem_Collect_eq reach_commit_order_complete txid0.exhaust).
-  next
-    case (WCommit x1 x2 x3 x4 x5)
-    then show ?case apply (simp add: Commit_Order_Superset_View_def tps_trans_defs get_view_def)
-      apply (cases "x2 k", simp_all)
-      apply (rule subsetI) subgoal for x apply (cases x, blast)
-        by (smt mem_Collect_eq Commit_Order_Complete_def reach_commit_order_complete txid0.exhaust)
-      apply (rule allI) subgoal for _ cl apply (cases "cl = x1", simp)
-        apply (rule subsetI) subgoal for x apply (cases x, blast)
-          by (smt list.set_intros(2) list.simps(15) mem_Collect_eq Commit_Order_Complete_def
-              reach_commit_order_complete txid0.exhaust)
-        by blast.
-  qed (simp_all add: Commit_Order_Superset_View_def tps_trans_defs)
+        by (smt mem_Collect_eq reach_commit_order_complete txid0.exhaust)
+      subgoal for x apply (cases x)
+        apply blast using Commit_Order_Complete_def[of s k] sorry.
+  qed (auto simp add: Commit_Order_Superset_Ctx_def tps_trans_defs)
 qed
 
 definition Commit_Order_Superset_Get_View where
-  "Commit_Order_Superset_Get_View s k \<longleftrightarrow> (\<forall>cl. (get_view s cl) k \<subseteq> set (commit_order s k))"
+  "Commit_Order_Superset_Get_View s k \<longleftrightarrow> (\<forall>cl t. (k, t) \<in> get_view s cl \<longrightarrow> t \<in> set (commit_order s k))"
 
 lemmas Commit_Order_Superset_Get_ViewI = Commit_Order_Superset_Get_View_def[THEN iffD2, rule_format]
 lemmas Commit_Order_Superset_Get_ViewE[elim] = Commit_Order_Superset_Get_View_def[THEN iffD1, elim_format, rule_format]
@@ -1759,17 +1763,18 @@ next
   case (reach_trans s e s')
   then show ?case using get_view_inv[of s e s']
   proof (induction e)
-    case (CommitW x1 x2 x3 x4)
+    case (CommitW x1 x2 x3 x4 x5)
     then show ?case
       apply (simp add: Commit_Order_Superset_Get_View_def tps_trans_defs get_view_def)
-      apply (rule, rule, rule) subgoal for cl x apply (cases "x = x2"; auto)
+      apply (rule, rule, rule)
+      subgoal for cl x apply (cases "x = x2"; auto)
         using Gst_lt_Cts_def linorder_not_less reach_gst_lt_cts apply blast
           apply (cases x, blast)
         subgoal for kv_map y x2a apply (cases x2a)
           using Commit_Order_Complete_def[of s x1]
           by (metis (no_types, lifting) get_cl_wtxn.simps(2) get_sn_wtxn.simps(2)
               is_prepared.elims(2) reach_commit_order_complete is_curr_wt_def)
-        by blast+.
+        done.
   qed (simp_all add: Commit_Order_Superset_Get_View_def tps_trans_defs get_view_def, (blast+)?)
 qed
 
@@ -1835,7 +1840,7 @@ next
     case (PrepW x1 x2 x3)
     then show ?case sorry
   next
-    case (CommitW x1 x2 x3 x4)
+    case (CommitW x1 x2 x3 x4 x5)
     then show ?case sorry
   qed simp
 qed
@@ -1851,7 +1856,7 @@ lemma v_writer_set_commit_order_eq:
    apply (metis (mono_tags, lifting) is_committed.cases version.select_convs(2))
    subgoal for t apply (cases "wtxn_state (svrs s k) t", simp)
       apply (metis (opaque_lifting) ver_state.distinct(5) ver_state.inject(1) version.select_convs(2))
-     subgoal for cts v rs apply (rule exI[where x="\<lparr>v_value = v, v_writer = t,
+     subgoal for cts v rs deps apply (rule exI[where x="\<lparr>v_value = v, v_writer = t,
           v_readerset = {t \<in> rs. get_sn_txn t < txn_sn (cls s (get_cl_txn t))}\<rparr>"], simp)
        by (rule bexI[where x=t], auto)
      done.
@@ -1928,14 +1933,14 @@ next
     hence "\<And>k. prefix (commit_order s k) (commit_order s' k)" by (simp add: write_commit_def)
     hence "view_of (commit_order s') (get_view s cl) = view_of (commit_order s) (get_view s cl)"
       using WCommit view_of_prefix[of "commit_order s" "commit_order s'" "get_view s cl"]
-        Commit_Order_Distinct_def[of s'] Commit_Order_Superset_Get_View_def[of s]
-      by (metis reach.reach_trans reach_commit_order_distinct reach_commit_order_superset_get_view)
+        Commit_Order_Distinct_def[of s'] Commit_Order_Superset_Get_View_def[of s] sorry
+        (*by (metis reach.reach_trans reach_commit_order_distinct reach_commit_order_superset_get_view)*)
     hence "view_of (commit_order s') (get_view s' cl) = view_of (commit_order s) (get_view s cl)"
       using WCommit by (auto simp add: write_commit_def get_view_def)
     then show ?case using WCommit
       apply (simp add: Get_view_Wellformed_def tps_trans_defs) sorry
   next
-    case (CommitW x1 x2 x3 x4)
+    case (CommitW x1 x2 x3 x4 x5)
     then show ?case sorry
   qed (auto simp add: Get_view_Wellformed_def tps_trans_defs)
 qed
@@ -2057,7 +2062,7 @@ next
     case (PrepW x1 x2 x3)
     then show ?case apply (auto simp add: Disjoint_RW_def tps_trans_defs) sorry
   next
-    case (CommitW x1 x2 x3 x4)
+    case (CommitW x1 x2 x3 x4 x5)
     then show ?case sorry
   qed (auto simp add: Disjoint_RW_def tps_trans_defs)
 qed
@@ -2224,7 +2229,7 @@ next
     case (WCommit x1 x2 x3 x4 x5)
     then show ?case sorry
   next
-    case (CommitW x1 x2 x3 x4)
+    case (CommitW x1 x2 x3 x4 x5)
     then show ?case sorry
   qed (auto simp add: Get_view_Closed_def tps_trans_defs)
 qed
@@ -2252,7 +2257,7 @@ next
     case (PrepW x1 x2 x3)
     then show ?case sorry
   next
-    case (CommitW x1 x2 x3 x4)
+    case (CommitW x1 x2 x3 x4 x5)
     then show ?case sorry
   qed (auto simp add: RO_WO_Inv_def tps_trans_defs)
 qed
@@ -2260,10 +2265,10 @@ qed
 
 subsection \<open>View invariants\<close>
 
-lemma cl_view_inv:
+lemma cl_ctx_inv:
   assumes "state_trans s e s'"
     and "not_committing_ev e"
-  shows "cl_view (cls s' cl) = cl_view (cls s cl)"
+  shows "cl_ctx (cls s' cl) = cl_ctx (cls s cl)"
   using assms
   by (induction e) (auto simp add: tps_trans_defs views_of_s_def)
 
@@ -2298,7 +2303,7 @@ next
   case (PrepW x1 x2 x3)
   then show ?case sorry
 next
-  case (CommitW x1 x2 x3 x4)
+  case (CommitW x1 x2 x3 x4 x5)
   then show ?case sorry
 qed simp
 
@@ -2326,7 +2331,7 @@ proof(induction s rule: reach.induct)
   case (reach_init s)
   then show ?case
     by (auto simp add: Views_of_s_Wellformed_def tps_defs view_of_def views_of_s_def the_T0
-        view_txid_init_def view_wellformed_defs full_view_def kvs_of_s_def)
+        ctx_kt_init_def view_wellformed_defs full_view_def kvs_of_s_def)
 next
   case (reach_trans s e s')
   then show ?case using kvs_of_s_inv[of s e s'] views_of_s_inv[of s e s']
@@ -2344,24 +2349,23 @@ subsection \<open>View Shift\<close>
 
 lemma get_view_grows:
   assumes "state_trans s e s'" and "Gst_le_Min_Lst_map s cl"
-  shows "get_view s cl \<sqsubseteq> get_view s' cl"
+  shows "(\<lambda>k. get_view s cl `` {k}) \<sqsubseteq> (\<lambda>k. get_view s' cl `` {k})"
   using assms get_view_inv[of s e s']
   by (induction e) (auto simp add: tps_trans_defs view_order_def get_view_def)
 
-definition Cl_View_WtxnCommit where
-  "Cl_View_WtxnCommit s cl \<longleftrightarrow>
-    (\<forall>cts kv_map k. txn_state (cls s cl) = WtxnCommit cts kv_map \<longrightarrow>
-      cl_view (cls s cl) k = (case kv_map k of None \<Rightarrow> get_view s cl k |
-        Some _ \<Rightarrow> insert (get_wtxn_cl s cl) (get_view s cl k)))"
+definition Cl_Ctx_WtxnCommit where
+  "Cl_Ctx_WtxnCommit s cl \<longleftrightarrow>
+    (\<forall>cts kv_map deps k. txn_state (cls s cl) = WtxnCommit cts kv_map deps \<and> k \<in> dom kv_map \<longrightarrow>
+      (k, get_wtxn_cl s cl) \<in> cl_ctx (cls s cl))"
 
-lemmas Cl_View_WtxnCommitI = Cl_View_WtxnCommit_def[THEN iffD2, rule_format]
-lemmas Cl_View_WtxnCommitE[elim] = Cl_View_WtxnCommit_def[THEN iffD1, elim_format, rule_format]
+lemmas Cl_Ctx_WtxnCommitI = Cl_Ctx_WtxnCommit_def[THEN iffD2, rule_format]
+lemmas Cl_Ctx_WtxnCommitE[elim] = Cl_Ctx_WtxnCommit_def[THEN iffD1, elim_format, rule_format]
 
-lemma reach_cl_view_wtxncommit [simp]: "reach tps s \<Longrightarrow> Cl_View_WtxnCommit s cl"
+lemma reach_cl_ctx_wtxncommit [simp]: "reach tps s \<Longrightarrow> Cl_Ctx_WtxnCommit s cl"
 proof(induction s rule: reach.induct)
   case (reach_init s)
   then show ?case
-    by (auto simp add: Cl_View_WtxnCommit_def tps_defs)
+    by (auto simp add: Cl_Ctx_WtxnCommit_def tps_defs)
 next
   case (reach_trans s e s')
   then show ?case using get_view_inv[of s e s']
@@ -2369,15 +2373,15 @@ next
     case (RInvoke x1 x2)
     then show ?case sorry
   next
-    case (CommitW x1 x2 x3 x4)
+    case (CommitW x1 x2 x3 x4 x5)
     then show ?case sorry
-  qed (auto simp add: Cl_View_WtxnCommit_def tps_trans_defs split: option.split)
+  qed (auto simp add: Cl_Ctx_WtxnCommit_def tps_trans_defs split: option.split)
 qed
 
 definition Cl_Sub_Get_View where
   "Cl_Sub_Get_View s cl \<longleftrightarrow>
-    (\<forall>keys kv_map. txn_state (cls s cl) \<in> {Idle, RtxnInProg keys kv_map, WtxnPrep kv_map} \<longrightarrow>
-      cl_view (cls s cl) \<sqsubseteq> get_view s cl)"
+    (\<forall>keys kvt_map kv_map. txn_state (cls s cl) \<in> {Idle, RtxnInProg keys kvt_map, WtxnPrep kv_map} \<longrightarrow>
+      cl_ctx (cls s cl) \<subseteq> get_view s cl)"
 
 lemmas Cl_Sub_Get_ViewI = Cl_Sub_Get_View_def[THEN iffD2, rule_format]
 lemmas Cl_Sub_Get_ViewE[elim] = Cl_Sub_Get_View_def[THEN iffD1, elim_format, rule_format]
@@ -2386,23 +2390,22 @@ lemma reach_cl_sub_get_view [simp]: "reach tps s \<Longrightarrow> Cl_Sub_Get_Vi
 proof(induction s rule: reach.induct)
   case (reach_init s)
   then show ?case
-    by (auto simp add: Cl_Sub_Get_View_def tps_defs version_order_def view_txid_init_def get_view_def)
+    by (auto simp add: Cl_Sub_Get_View_def tps_defs version_order_def ctx_kt_init_def get_view_def)
 next
   case (reach_trans s e s')
   then show ?case using get_view_inv[of s e s']
   proof (induction e)
     case (RInvoke x1 x2)
-    then show ?case apply (simp add: Cl_Sub_Get_View_def tps_trans_defs)
-      by (metis get_view_grows reach_gst_le_min_lst_map reach_trans.hyps(1) tps_trans
-          view_order_transitive)
+    then show ?case apply (simp add: Cl_Sub_Get_View_def tps_trans_defs) sorry
+      (*by (metis get_view_grows reach_gst_le_min_lst_map reach_trans.hyps(1) tps_trans
+          view_order_transitive)*)
   next
     case (WDone x1 x2)
-    then show ?case apply (auto simp add: Cl_Sub_Get_View_def tps_trans_defs get_view_def view_order_def) sorry
+    then show ?case (*apply (auto simp add: Cl_Sub_Get_View_def tps_trans_defs get_view_def view_order_def)*) sorry
   next
-    case (CommitW x1 x2 x3 x4)
-    then show ?case apply (auto simp add: Cl_Sub_Get_View_def tps_trans_defs) sorry
-  qed (auto simp add: Cl_Sub_Get_View_def tps_trans_defs)
-qed
+    case (CommitW x1 x2 x3 x4 x5)
+    then show ?case (*apply (auto simp add: Cl_Sub_Get_View_def tps_trans_defs)*) sorry
+    oops(***)
 
 lemma read_commit_added_txid:
   assumes "read_done cl kv_map sn u s s'"
@@ -2413,31 +2416,31 @@ lemma read_commit_added_txid:
 
 subsection \<open>View Grows\<close>
 
-lemma view_grows_view_of: "a \<sqsubseteq> b \<Longrightarrow> view_of corder a \<sqsubseteq> view_of corder b"
+lemma view_grows_view_of: "a \<subseteq> b \<Longrightarrow> view_of corder a \<sqsubseteq> view_of corder b"
   apply (simp add: view_of_def)
   by (smt (verit) Collect_mono_iff insert_subset mk_disjoint_insert view_order_def)
 
 definition View_Grows where
   "View_Grows s cl \<longleftrightarrow>
-    (\<forall>keys kv_map. txn_state (cls s cl) \<in> {Idle, RtxnInProg keys kv_map, WtxnPrep kv_map} \<longrightarrow>
+    (\<forall>keys kvt_map kv_map. txn_state (cls s cl) \<in> {Idle, RtxnInProg keys kvt_map, WtxnPrep kv_map} \<longrightarrow>
       views_of_s s cl \<sqsubseteq> view_of (commit_order s) (get_view s cl))"
 
 lemmas View_GrowsI = View_Grows_def[THEN iffD2, rule_format]
 lemmas View_GrowsE[elim] = View_Grows_def[THEN iffD1, elim_format, rule_format]
 
 lemma reach_view_grows [simp]: "reach tps s \<Longrightarrow> View_Grows s cl"
-  apply (simp add: View_Grows_def views_of_s_def)
-  by (metis view_grows_view_of Cl_Sub_Get_View_def insertI1 insertI2 reach_cl_sub_get_view)
+  apply (simp add: View_Grows_def views_of_s_def) oops
+  (*by (metis view_grows_view_of Cl_Sub_Get_View_def insertI1 insertI2 reach_cl_sub_get_view)*)
 
 section \<open>Fp Property\<close>
 
 \<comment> \<open>Fingerprint content invariant and Lemmas for proving the fp_property\<close>
 
 definition RegR_Fp_Inv where
-  "RegR_Fp_Inv s k \<longleftrightarrow> (\<forall>t keys kv_map cts v rs.
+  "RegR_Fp_Inv s k \<longleftrightarrow> (\<forall>t keys kv_map cts v rs deps.
     txn_state (cls s (get_cl_txn t)) = RtxnInProg keys kv_map \<and> k \<in> keys \<and> kv_map k = None \<and>
     wtxn_state (svrs s k) (read_at (wtxn_state (svrs s k)) (gst (cls s (get_cl_txn t))) (get_cl_txn t))
-       = Commit cts v rs \<longrightarrow>
+       = Commit cts v rs deps \<longrightarrow>
     v = v_value (last_version (kvs_of_s s k) (view_of (commit_order s) (get_view s (get_cl_txn t)) k)))"
 
 lemmas RegR_Fp_InvI = RegR_Fp_Inv_def[THEN iffD2, rule_format]
@@ -2469,14 +2472,14 @@ next
     case (PrepW x1 x2 x3)
     then show ?case apply (auto simp add: RegR_Fp_Inv_def tps_trans_defs) sorry
   next
-    case (CommitW x1 x2 x3 x4)
+    case (CommitW x1 x2 x3 x4 x5)
     then show ?case sorry
   qed (auto simp add: RegR_Fp_Inv_def tps_trans_defs)
 qed
 
 definition Rtxn_Fp_Inv where
-  "Rtxn_Fp_Inv s cl \<longleftrightarrow> (\<forall>keys kv_map k v. txn_state (cls s cl) = RtxnInProg keys kv_map \<and>
-    kv_map k = Some v \<longrightarrow>
+  "Rtxn_Fp_Inv s cl \<longleftrightarrow> (\<forall>keys kvt_map k v t. txn_state (cls s cl) = RtxnInProg keys kvt_map \<and>
+    kvt_map k = Some (v, t) \<longrightarrow>
       v = v_value (last_version (kvs_of_s s k) (view_of (commit_order s) (get_view s cl) k)))"
 
 lemmas Rtxn_Fp_InvI = Rtxn_Fp_Inv_def[THEN iffD2, rule_format]
@@ -2502,7 +2505,7 @@ next
     case (WCommit x1 x2 x3 x4 x5)
     then show ?case sorry
   next
-    case (CommitW x1 x2 x3 x4)
+    case (CommitW x1 x2 x3 x4 x5)
     then show ?case sorry
   qed (auto simp add: Rtxn_Fp_Inv_def tps_trans_defs)
 qed
@@ -2510,7 +2513,7 @@ qed
 
 abbreviation invariant_list where
   "invariant_list s \<equiv> (\<forall>cl. invariant_list_kvs s \<and> Sqn_Inv_c s cl \<and> Sqn_Inv_nc s cl \<and> Get_view_Closed s cl
-    \<and>  Get_view_Wellformed s cl \<and> Views_of_s_Wellformed s cl \<and> View_Grows s cl \<and> Rtxn_Fp_Inv s cl)"
+    \<and>  Get_view_Wellformed s cl \<and> Views_of_s_Wellformed s cl \<and> Rtxn_Fp_Inv s cl)" (*\<and> View_Grows s cl*)
 
 
 section \<open>Refinement Proof\<close>
@@ -2521,7 +2524,7 @@ proof (intro simulate_ES_fun)
   assume p: "init tps gs0"
   then show "init ET_CC.ET_ES (sim gs0)"
     by (auto simp add: ET_CC.ET_ES_defs tps_defs sim_defs kvs_init_def v_list_init_def version_init_def
-        view_txid_init_def view_of_def the_T0)
+        ctx_kt_init_def view_of_def the_T0)
 next
   fix gs a and gs' :: "'v state"
   assume p: "tps: gs\<midarrow>a\<rightarrow> gs'" and reach_s: "reach tps gs" and "reach ET_CC.ET_ES (sim gs)"
@@ -2532,26 +2535,31 @@ next
     case (RDone cl kv_map sn u'')
     then show ?case
     apply (auto simp add: read_done_def sim_def intro!: exI [where x="views_of_s gs' cl"])
-    subgoal apply (auto simp add: ET_CC.ET_cl_txn_def t_is_fresh KvsOfS_Not_Emp_def Get_view_Closed_def)
-      subgoal by (metis Views_of_s_Wellformed_def p reach_s reach_trans reach_views_of_s_wellformed)                   
+      subgoal apply (auto simp add: ET_CC.ET_cl_txn_def t_is_fresh KvsOfS_Not_Emp_def Get_view_Closed_def)
+        subgoal (* updated ctx wellformed *) sorry
+        subgoal by (metis Views_of_s_Wellformed_def p reach_s reach_trans reach_views_of_s_wellformed)                   
+        subgoal (* canCommit *) sorry
       subgoal apply (auto simp add: vShift_MR_RYW_def vShift_MR_def vShift_RYW_def views_of_s_def)
         \<comment> \<open>1. view_of corder get_view \<sqsubseteq> view_of corder' cl_view'
             2. (writer_ver_i, t) \<in> SO \<Longrightarrow> t \<in> K'\K \<Longrightarrow> i \<in> view_of corder' cl_view'
             3. writer_ver_i \<in> K'\K \<Longrightarrow> i \<in> view_of corder' cl_view'\<close>
+        subgoal by (simp add: read_done_s'_def) (* view grows not needed anymore*)
         sorry
-      subgoal using View_Grows_def insert_compr mem_Collect_eq by blast
+      subgoal by (simp add: views_of_s_def view_grows_view_of)
       subgoal sorry
       done
       subgoal by (rule ext, simp add: read_done_def views_of_s_def read_done_s'_def)
-      subgoal apply (auto simp add: fp_property_def view_snapshot_def) by blast.
+      subgoal apply (auto simp add: fp_property_def view_snapshot_def) sorry (* need alternative for Rtxn_Fp_Inv *).
   next
     case (WCommit cl kv_map cts sn u'')
     then show ?case
     apply (auto simp add: write_commit_def sim_def fp_property_def intro!: exI [where x="views_of_s gs' cl"])
       subgoal apply (auto simp add: ET_CC.ET_cl_txn_def t_is_fresh Get_view_Closed_def)
+        subgoal (* updated ctx wellformed *) sorry
         subgoal by (metis Views_of_s_Wellformed_def p reach_s reach_trans reach_views_of_s_wellformed)
+        subgoal (* canCommit *)  sorry
         subgoal sorry
-        subgoal using View_Grows_def insert_compr mem_Collect_eq by blast
+        subgoal by (simp add: views_of_s_def view_grows_view_of) 
         subgoal sorry
         done
     subgoal apply (rule ext)
